proof/SubtypingSimp.v
@@ -16,7 +16,6 @@ From Coq Require Import Lists.List.
 Import CoreLangSimp.
 Import LinearContext.
 Import TermOrdering.
-Import Nstate.
 Import TypeClosedSimp.
 Import DenotationSimp.
 Import TermMeet.
@@ -24,40 +23,43 @@ Import DenotationAux.
 Import WellFormedSimp.
 Import ListNotations.
 
-Inductive tmR_sub_in_ctx_aux: nstate -> context -> overunderty -> overunderty -> Prop :=
-| tmR_sub_in_ctx_aux_nil: forall (nst: nstate) (tau1 tau2: underty),
+Inductive tmR_sub_in_ctx_aux: state -> context -> overunderty -> overunderty -> Prop :=
+| tmR_sub_in_ctx_aux_nil: forall (nst: state) (tau1 tau2: underty),
     well_formed_type tau1 -> well_formed_type tau2 ->
     u\_ tau1 _/ = u\_ tau2 _/ ->
     (forall e, tmR_in_ctx_aux nst [] tau1 e -> tmR_in_ctx_aux nst [] tau2 e) ->
     tmR_sub_in_ctx_aux nst [] tau1 tau2
 | tmR_sub_in_ctx_aux_cons_overbase:
-  forall (nst: nstate) (x: string) (T:base_ty) (phi: refinement) (Gamma: context) (tau1 tau2: underty),
+  forall (nst: state) (x: string) (T:base_ty) (phi: refinement) (Gamma: context) (tau1 tau2: underty),
     nst x = None ->
     l_find_right_most Gamma x = None ->
     well_formed_type tau1 -> well_formed_type tau2 ->
     well_formed_type ({{v: T | phi}}) ->
     (forall (c_x: constant), tmR_aux nst ({{v: T | phi}}) c_x ->
-                        tmR_sub_in_ctx_aux (update nst x (tvalue c_x, T)) Gamma tau1 tau2) ->
+                        tmR_sub_in_ctx_aux (update nst x c_x) Gamma tau1 tau2) ->
     u\_ tau1 _/ = u\_ tau2 _/ ->
     tmR_sub_in_ctx_aux nst ((x, (Oty ({{v: T | phi}}))) :: Gamma) tau1 tau2
 | tmR_sub_in_ctx_aux_cons_under:
-  forall (nst: nstate) (x: string) (T:base_ty) (phi: refinement) (Gamma: context) (tau1 tau2: underty),
+  forall (nst: state) (x: string) (T:base_ty) (phi: refinement) (Gamma: context) (tau1 tau2: underty),
     nst x = None ->
     l_find_right_most Gamma x = None ->
     well_formed_type tau1 -> well_formed_type tau2 ->
     well_formed_type ([[v: T | phi]]) ->
     (exists e_x_hat, tmR_aux nst ([[v: T | phi]]) e_x_hat /\
-                  tmR_sub_in_ctx_aux (update nst x (e_x_hat, T)) Gamma tau1 tau2) ->
+                  (forall e_x, tmR_aux nst ([[v: T | phi]]) e_x ->
+                          (forall (v_x_hat: constant), e_x -->* v_x_hat ->
+                                                  tmR_sub_in_ctx_aux (update nst x v_x_hat) Gamma tau1 tau2
+    ))) ->
     u\_ tau1 _/ = u\_ tau2 _/ ->
     tmR_sub_in_ctx_aux nst ((x, (Uty ([[v: T | phi]]))) :: Gamma) tau1 tau2
-| tmR_sub_in_ctx_aux_cons_oarr: forall (nst: nstate) (x: string) a T phi (tau_b: underty) (Gamma: context) (tau1 tau2: underty),
+| tmR_sub_in_ctx_aux_cons_oarr: forall (nst: state) (x: string) a T phi (tau_b: underty) (Gamma: context) (tau1 tau2: underty),
     nst x = None ->
     l_find_right_most Gamma x = None ->
     well_formed_type tau1 -> well_formed_type tau2 ->
     well_formed_type (a o: {{v: T | phi}} o--> tau_b) ->
     tmR_sub_in_ctx_aux nst Gamma tau1 tau2 ->
     tmR_sub_in_ctx_aux nst ((x, Uty (a o: ({{v: T | phi}}) o--> tau_b)) :: Gamma) tau1 tau2
-| tmR_sub_in_ctx_aux_cons_underarr: forall (nst: nstate) (x: string) (t1 t2: underty) (Gamma: context) (tau1 tau2: overunderty),
+| tmR_sub_in_ctx_aux_cons_underarr: forall (nst: state) (x: string) (t1 t2: underty) (Gamma: context) (tau1 tau2: overunderty),
     nst x = None ->
     l_find_right_most Gamma x = None ->
     well_formed_type tau1 -> well_formed_type tau2 ->
@@ -114,13 +116,45 @@ Proof with eauto.
   induction H; simpl...
 Qed.
 
-Lemma term_order_implies_subtyping_order: forall e_x_hat e_x_hat1 T a st Gamma tau12 tau22,
-    e_x_hat <-< e_x_hat1 ->
-    tmR_sub_in_ctx_aux (a |-> (e_x_hat1, T); st) Gamma tau12 tau22 ->
-    tmR_sub_in_ctx_aux (a |-> (e_x_hat, T); st) Gamma tau12 tau22.
-Admitted.
+(* Lemma term_order_implies_subtyping_order: forall Gamma e e' T x st (tau1 tau2: underty), *)
+(*     e <-< e' -> *)
+(*     tmR_sub_in_ctx_aux (x |-> (e', T); st) Gamma tau1 tau2 -> *)
+(*     tmR_sub_in_ctx_aux (x |-> (e, T); st) Gamma tau1 tau2. *)
+(* Proof with eauto. *)
+(*   intros Gamma. *)
+(*   induction Gamma; simpl; intros e e' T x st tau1 tau2 Hts H1. *)
+(*   - inversion H1; subst... constructor... intros ee HeeD. *)
+(*     eapply term_order_implies_state_order... eapply H6... *)
+(* Admitted. *)
 
-Global Hint Resolve term_order_implies_subtyping_order: core.
+(* Global Hint Resolve term_order_implies_subtyping_order: core. *)
+
+(* Lemma step_preserve_ctx_denotation: forall Gamma (e e': tm), *)
+(*     e <-< e' -> (forall st (tau: underty), tmR_in_ctx_aux st Gamma tau e -> tmR_in_ctx_aux st Gamma tau e'). *)
+(* Proof with eauto. *)
+(*   intros Gamma. *)
+(*   induction Gamma; simpl; intros e e' Hts st tau He... *)
+(*   - rewrite tmR_in_ctx_to_under. rewrite tmR_in_ctx_to_under in He. eapply step_preserve_under_denotation... *)
+(*   - inversion He; subst. *)
+(*     + constructor... *)
+(*       intros c_x Hc_xD. assert (tmR_in_ctx_aux (x |-> c_x; st) Gamma tau (tlete x c_x e)) as Hv1... *)
+(*       eapply IHGamma... apply eta_self1... *)
+(*     + constructor... *)
+(*       destruct H8 as (e_x_hat & He_x_hatD & HH). *)
+(*       exists e_x_hat. split... *)
+(*       intros e_x He_xD. *)
+(*       assert (tmR_in_ctx_aux (x |-> (e_x_hat, T); st) Gamma tau (tlete x e_x e))... *)
+(*       eapply IHGamma... apply eta_self1... *)
+(*     + constructor... *)
+(*       intros e_x He_xD. *)
+(*       assert (tmR_in_ctx_aux st Gamma tau (tlete x e_x e))... *)
+(*       eapply IHGamma... apply eta_self1... *)
+(*     + constructor... *)
+(*       intros e_x He_xD. *)
+(*       assert (tmR_in_ctx_aux st Gamma tau (tlete x e_x e))... *)
+(*       eapply IHGamma... apply eta_self1... *)
+(* Qed. *)
+
 
 Lemma subtyping_soundness_arrarr: forall Gamma st tau11 tau12 tau21 tau22,
     u\_ tau21 _/ = u\_ tau11 _/ -> u\_ tau12 _/ = u\_ tau22 _/ ->
@@ -146,23 +180,22 @@ Proof with eauto.
       destruct (meet_of_two_terms_exists e_x_hat1 e_x_hat2 T) as (e_x_hat & HT & HE); try tmR_implies_has_type...
       constructor...
       exists e_x_hat... split. eapply meet_of_two_terms_implies_denotation in HE...
-      apply meet_of_two_terms_term_order in HE... destruct HE as (HEE1 & HEE2).
-      apply IHGamma... simpl. rewrite H11... rewrite H19...
+      intros e_x He_xD v_x_hat HvE. apply IHGamma... simpl. rewrite H11... rewrite H19...
     + inversion Hsub2; subst...
     + inversion Hsub2; subst...
 Qed.
 
-Lemma subtype_over_sub_phi: forall st T phi11 phi21,
-  (forall c, phi_sat_nst phi21 st c -> phi_sat_nst phi11 st c) ->
-  (forall c : constant, overbase_tmR_aux st ({{v:T | phi21}}) c -> overbase_tmR_aux st ({{v:T | phi11}}) c).
+Lemma subtype_over_sub_phi: forall st T (phi11 phi21: refinement),
+    (forall c, phi21 st c -> phi11 st c) ->
+    (forall c : constant, overbase_tmR_aux st ({{v:T | phi21}}) c -> overbase_tmR_aux st ({{v:T | phi11}}) c).
 Proof with eauto.
   intros.
   inversion H0; subst.
   constructor...
 Qed.
 
-Lemma subtype_under_sub_phi: forall st T phi11 phi21,
-  (forall c, phi_sat_nst phi21 st c -> phi_sat_nst phi11 st c) ->
+Lemma subtype_under_sub_phi: forall st T (phi11 phi21: refinement),
+  (forall c, phi21 st c -> phi11 st c) ->
   (forall e : tm, under_tmR_aux st ([[v:T | phi11]]) e -> under_tmR_aux st ([[v:T | phi21]]) e).
 Proof with eauto.
   intros.
@@ -192,7 +225,7 @@ Proof with eauto.
     rewrite tmR_in_ctx_to_under. rewrite tmR_in_ctx_to_under in H. inversion Hsub1; subst.
     (* inversion Hsub2; subst. *)
     (* constructor... split... simpl. rewrite <- HeqT... apply under_tmR_has_type in H... *)
-    (* intros. inversion H1; subst. simpl. assert (tmR_sub_in_ctx_aux (x |-> (tvalue c_x, T); st) [] tau12 tau22)... *)
+    (* intros. inversion H1; subst. simpl. assert (tmR_sub_in_ctx_aux (x |-> c_x; st) [] tau12 tau22)... *)
     (* inversion H7; subst. setoid_rewrite tmR_in_ctx_to_under in H15. apply H15... *)
     (* inversion H; subst. destruct H17. apply H18... setoid_rewrite tmR_aux_to_over in Hsub1... *)
   - destruct a as (a & tau_a).
@@ -240,41 +273,12 @@ Proof with eauto.
       destruct (meet_of_two_terms_exists e_x_hat1 e_x_hat2 T) as (e_x_hat & HT & HE); try tmR_implies_has_type...
       constructor...
       exists e_x_hat... split. eapply meet_of_two_terms_implies_denotation in HE...
-      intros e_x He_xD.
-      apply meet_of_two_terms_term_order in HE... destruct HE as (HEE1 & HEE2).
+      intros e_x He_xD v_x_hat HvE.
+      (* apply meet_of_two_terms_term_order in HE... destruct HE as (HEE1 & HEE2). *)
       eapply IHGamma...
     + inversion He1; subst...
     + inversion He1; subst...
 Qed.
-
-(* Lemma subtyping_denotation_implies_denotation_base_rev: forall Gamma st T phi1 phi2 , *)
-(*     (forall e, tmR_in_ctx_aux st Gamma ([[v: T | phi1]]) e -> tmR_in_ctx_aux st Gamma ([[v: T | phi2]]) e) -> *)
-(*     tmR_sub_in_ctx_aux st Gamma ([[v: T | phi1]]) ([[v: T | phi2]]). *)
-(* Proof with eauto. *)
-(*   intro Gamma. *)
-(*   induction Gamma; simpl; intros st T phi1 phi2 HD... *)
-(*   - destruct a as (a & tau_a). *)
-(*     destruct tau_a. *)
-(*     admit. destruct o. *)
-(*     constructor... admit. admit. intros c_x Hc_xD. *)
-(*     admit. *)
-(*   -  *)
-(*   - *)
-(*   - inversion HD; subst... *)
-(*   - inversion HD; subst... *)
-(*     + inversion He1; subst. constructor... *)
-(*     + inversion He1; subst. *)
-(*       destruct H9 as (e_x_hat1 & He_x_hat1D & HH1). *)
-(*       destruct H16 as (e_x_hat2 & He_x_hat2D & HH2). *)
-(*       destruct (meet_of_two_terms_exists e_x_hat1 e_x_hat2 T) as (e_x_hat & HT & HE); try tmR_implies_has_type... *)
-(*       constructor... *)
-(*       exists e_x_hat... split. eapply meet_of_two_terms_implies_denotation in HE... *)
-(*       intros e_x He_xD. *)
-(*       apply meet_of_two_terms_term_order in HE... destruct HE as (HEE1 & HEE2). *)
-(*       eapply IHGamma... *)
-(*     + inversion He1; subst... *)
-(*     + inversion He1; subst... *)
-(* Qed *)
 
 Lemma is_subtype_spec: forall Gamma t1 t2,
     is_subtype Gamma t1 t2 ->
@@ -283,36 +287,3 @@ Proof with eauto.
   intros. apply subtyping_soundness in H.
   eapply subtyping_denotation_implies_denotation_base...
 Qed.
-
-(* Lemma tmR_empty_under: forall st (tau11: underty) e, *)
-(*   tmR_in_ctx_aux st [] tau11 e <-> under_tmR_aux st tau11 e. *)
-(* Admitted. *)
-
-(* Lemma tmR_empty_implies_forall_state: forall Gamma tau e, *)
-(*     (forall st, tmR_in_ctx_aux st Gamma tau e) <-> tmR_in_ctx_aux empty Gamma tau e. *)
-(* Admitted. *)
-
-(* Lemma subtyping_arrarr: forall Gamma st (t1 t2: underty) e, *)
-(*     ctx_inv st Gamma -> *)
-(*     (forall e_x, tmR_in_ctx_aux st Gamma t1 e_x -> *)
-(*             (forall e3, is_application e e_x e3 -> tmR_in_ctx_aux st Gamma t2 e3)) -> *)
-(*     (tmR_in_ctx_aux st Gamma (t1 u--> t2) e). *)
-(* Proof with eauto. *)
-(*   intro Gamma. *)
-(*   induction Gamma; simpl; intros st t1 t2 e Hinv He... *)
-(*   - admit. *)
-(*   - destruct a as (a, tau_a). assert (well_formed_type tau_a). admit. *)
-(*     destruct tau_a. admit. destruct o. *)
-(*     constructor... admit. admit. *)
-(*     intros c_x Hc_xD. *)
-(*     eapply IHGamma...  intros. inversion H1; subst... clear H1. *)
-(*     assert (tmR_in_ctx_aux (a |-> (c_x, b); st) Gamma (t1 u--> t2) (tlete a c_x e)). *)
-(*     apply IHGamma... intros e_x He_xD e3 Happ. *)
-
-(*     assert (tmR_in_ctx_aux st ((a, Oty ({{v:b | r}})) :: Gamma) t2 e3). eapply He with (e_x:= (tlete a c_x e_x))... *)
-
-
-(*     destruct Hinv. ctx_inv. destruct a as (a, tau_a). *)
-
-
-(*     constructor... admit. *)
